Encoding: Refactoring nach Typeclasses, Verstärkung der Korrekheit
TODO: Listen-Decodierung

TM/Encoding.v
@@ -1,112 +1,27 @@
-Require Import Prelim LiftNM Compound.
-
-(** * Coding Alphabet *)
-
-Notation "'codsig'" := (bool).
-
-(** * Coding Types **)
-
-Inductive codtype : Type :=
-| codtuple : forall (t1 t2 : codtype), codtype
-| codlist  : forall (t : codtype), codtype
-| codsum   : forall (t1 t2 : codtype), codtype
-| codunit  : codtype.
-
-Instance codtype_dec : eq_dec codsig.
-Proof. intros x y. hnf. decide equality. Defined.
-
-(** Compound Types *)
-Definition codnat := codlist codunit.
-Definition codbool := codsum codunit codunit.
-Definition codopt (t : codtype) := codsum t codunit.
-Definition codtriple (t1 t2 t3 : codtype) := codtuple (codtuple t1 t2) t3.
-
-Fixpoint codtype_to_type (t : codtype) : Type :=
-  match t with
-  | codtuple t1 t2 => prod (codtype_to_type t1) (codtype_to_type t2)
-  | codlist  t     => list (codtype_to_type t)
-  | codsum   t1 t2 => sum  (codtype_to_type t1) (codtype_to_type t2)
-  | codunit        => unit
-  end.
-
-
-(** * Encoding *)
-
-Definition encoding_function (t : codtype) :=
-  forall v : codtype_to_type t, list codsig.
-
-Fixpoint encode_list (t : codtype) (encode_entries : encoding_function t) (xs : list (codtype_to_type t)) : list codsig.
-Proof.
-  destruct xs.
-  - apply (false :: nil).
-  - apply (cons true). apply app. apply (encode_entries c). apply (encode_list t encode_entries xs).
-Defined.
-    
-Fixpoint encode (t : codtype) : codtype_to_type t -> list codsig.
-Proof.
-  destruct t; cbn.
-  - intros (a,b). apply (encode t1 a ++ encode t2 b).
-  - apply encode_list. intros v. apply (encode t v).
-  - intros [a|b].
-    + apply (true  :: encode t1 a).
-    + apply (false :: encode t2 b).
-  - intros _. apply nil.
-Defined.
-
-(** * Convert from Coq Type *)
-
-Definition from_bool (b : bool) := if b then inl tt else inr tt.
-Definition from_option (t : codtype) (o : option (codtype_to_type t)) :=
-  match o with Some d => inl d | None => inr tt end.
-Fixpoint from_nat n : (codtype_to_type codnat) :=
-  match n with
-  | S n' => tt :: from_nat n'
-  | O => nil
-  end.
-
-
-(** Test *)
-(*
-Compute @encode (codtuple (codopt codbool) codnat) (@from_option codbool (Some (from_bool false)), from_nat 3).
-Compute @encode (codtuple (codopt codbool) codnat) (@from_option codbool None, from_nat 3).
-*)
-
+Require Import Prelim.
 
 (** * Suffix *)
 
-Definition suffix (X : Type) (xs ys : list X) :=
-  exists n : nat, List.skipn n ys = xs.
+Inductive suffix (X : Type) : list X -> list X -> Type :=
+| suffix_full (xs : list X) : suffix xs xs
+| suffix_skip (xs ys : list X) (y : X) : suffix xs ys -> suffix xs (y :: ys).
+Hint Constructors suffix.
+
+Goal suffix [1;2;3] [4;5;6;1;2;3]. Proof. repeat constructor. Qed.
+
+Lemma suffix_skip' (X : Type) (x : X) (xs : list X) :
+  suffix xs (x :: xs).
+Proof. do 2 constructor. Qed.
 
 Lemma suffix_nil (X : Type) (xs : list X) : suffix [] xs.
-Proof.
-  induction xs.
-  - exists 0. reflexivity.
-  - destruct IHxs as (n&H). exists (S n). assumption.
-Qed.
-
-Lemma skipn_nil (X : Type) (n : nat) : skipn n (@nil X) = [].
-Proof. induction n; cbn in *; auto. Qed.
+Proof. induction xs; auto. Qed.
 
 Lemma suffix_from_nil (X : Type) (xs : list X) : suffix xs [] -> xs = [].
-Proof. intros (n&H). rewrite skipn_nil in H. congruence. Qed.
-
-Lemma skipn_plus (X : Type) (xs : list X) (n1 n2 : nat) :
-  skipn (n1 + n2) xs = skipn n2 (skipn n1 xs).
-Proof.
-  revert n2 xs. induction n1; intros n2 xs; cbn in *.
-  - reflexivity.
-  - destruct xs as [ | x xs]; cbn; auto. now rewrite skipn_nil.
-Qed.
+Proof. inversion 1; now subst. Qed.
 
 Lemma suffix_transitive (X : Type) (xs ys zs : list X) :
   suffix ys xs -> suffix zs ys -> suffix zs xs.
-Proof.
-  intros (n1&H1) (n2&H2). subst. eexists. now eapply skipn_plus.
-Qed.
-
-Lemma suffix_skip (X : Type) (xs ys : list X) (y : X) :
-  suffix xs ys -> suffix xs (y :: ys).
-Proof. intros (n&<-). exists (S n). cbn. reflexivity. Qed.
+Proof. intros H. revert zs. induction H; auto. Qed.
 
 Lemma suffix_app (X : Type) (xs ys zs : list X) :
   suffix xs ys -> suffix xs (zs ++ ys).
@@ -116,11 +31,6 @@ Proof.
   - cbn. apply suffix_skip. auto.
 Qed.
 
-Lemma suffix_full (X : Type) (xs : list X) :
-  suffix xs xs.
-Proof. now exists 0. Qed.
-
-
 Lemma list_con_neq (X : Type) (xs : list X) (x : X) :
   xs <> x :: xs.
 Proof.
@@ -129,70 +39,49 @@ Proof.
   - intros H. injection H. intros H' ->. congruence.
 Qed.
 
+Lemma list_app_neq (X : Type) (xs ys : list X) (y : X) :
+  xs <> y :: ys ++ xs.
+Proof. intros H. assert (|xs| = |y :: ys ++ xs|) as H' by congruence. cbn in *. rewrite app_length in H'. omega. Qed.
 
-Lemma skipn_size (X : Type) (xs : list X) (n : nat) : xs <> nil -> n > 0 -> | skipn n xs | < | xs |.
-Proof.
-  revert xs. induction n; intros xs H1; cbn in *.
-  - omega.
-  - destruct xs; cbn in *.
-    + tauto.
-    + decide (n = 0) as [-> | H3]; cbn in *.
-      * omega.
-      * assert (n > 0) as H4 by omega.
-        intros H.
-        assert (xs = [] \/ xs <> []) as [-> | H5].
-        { destruct xs; [left|right]; congruence. }
-        -- rewrite skipn_nil. cbn. omega.
-        -- specialize (IHn xs H5 H4). omega.
-Qed.
-
-Lemma suffix_put (X : Type) (xs : list X) (y : X) :
-  suffix (y :: xs) xs -> False.
-Proof.
-  intros (n&H). destruct n; cbn in *.
-  - now apply list_con_neq in H.
-  - destruct xs as [ | a xs ].
-    + congruence.
-    + assert ( | skipn (S n) (a :: xs ) | < | a :: xs |).
-      { apply skipn_size; subst. congruence. omega. }
-      cbn in H0. rewrite H in H0. cbn in *. omega.
-Qed.
-
-Lemma skipn_0 (X : Type) (n : nat) (xs : list X) :
-  skipn n xs = xs -> xs = nil \/ n = 0.
-Proof.
-  revert xs. induction n; intros xs H; cbn in *.
-  - auto.
-  - destruct xs.
-    + left. reflexivity.
-    + exfalso. eapply suffix_put; eexists. eauto.
-Qed.
+Lemma suffix_length (X : Type) (xs : list X) (ys : list X) :
+  suffix xs ys -> |xs| <= |ys|.
+Proof. induction 1; cbn; omega. Qed.
 
 Lemma suffix_size_decrease (X : eqType) (xs ys : list X) :
   xs <> ys -> suffix xs ys -> |xs| < |ys|.
 Proof.
-  intros H (n&H2). revert xs ys H H2.
-  induction n; intros xs ys H H2; cbn in *.
-  - subst. tauto.
-  - destruct ys.
-    + subst. tauto.
-    + subst. cbn in *.
-      decide (n = 0) as [-> | H1]; cbn in *.
-      * omega.
-      * decide (skipn n ys = ys) as [H2 | H2].
-        -- subst. specialize (IHn (skipn n ys) ys). destruct (skipn_0 H2) as [-> | ->]; cbn in *; auto.
-           rewrite skipn_nil. cbn. omega.
-        -- specialize (IHn (skipn n ys) ys H2). rewrite IHn. omega. reflexivity.
+  intros H. induction 1.
+  - tauto.
+  - cbn. decide (xs = ys) as [->|E].
+    + omega.
+    + rewrite IHX0. omega. assumption.
+Qed.
+
+Lemma suffix_put_app (X : eqType) (xs : list X) (ys : list X) :
+  ys <> nil -> suffix (ys ++ xs) xs -> False.
+Proof.
+  intros H H'. eapply suffix_size_decrease in H'.
+  assert ((|ys|) + (|xs|) < |xs|) as H'' by now rewrite <- app_length.
+  assert (|ys| > 0). destruct ys; cbn; omega. omega.
+  destruct ys; cbn in *. tauto. intros H''. eapply list_app_neq; eauto.
+Qed.
+
+Lemma suffix_put (X : eqType) (xs : list X) (y : X) :
+  suffix (y :: xs) xs -> False.
+Proof.
+  intros H. eapply suffix_size_decrease in H. cbn in *. omega.
+  intros H'. eapply list_con_neq; eauto.
 Qed.
 
 
-Inductive suffix_induction (ys : list codsig) : Type :=
-| suffix_induction_con : (forall xs: list codsig, suffix xs ys -> xs <> ys -> suffix_induction xs) ->
-                         suffix_induction ys.
+(** Suffix Induction *)
 
 Inductive size_ind (X : Type) (f : X -> nat) : X -> Type :=
 | size_ind_intro (x : X) : (forall y, f y < f x -> size_ind f y) -> size_ind f x.
 
+Inductive suffix_induction (X : Type) (ys : list X) : Type :=
+| suffix_induction_con : (forall xs: list X, suffix xs ys -> xs <> ys -> suffix_induction xs) ->
+                         suffix_induction ys.
 
 (* Opaque proofes for size_Ind *)
 Lemma nat_lt_0 (n : nat) : ~n < 0. Proof. omega. Qed.
@@ -207,89 +96,98 @@ Proof.
   - constructor. intros z C. apply IHn. eapply nat_lt_tran_S; eauto.
 Defined.
 
-Lemma suffix_induction_provider (ys : list codsig) : suffix_induction ys.
+Lemma suffix_induction_provider (X : eqType) (ys : list X) : suffix_induction ys.
 Proof.
-  pose proof (size_Ind (@List.length codsig) ys) as X. induction X as [ys _ IH].
+  pose proof (size_Ind (@List.length X) ys) as H. induction H as [ys _ IH].
   constructor. intros xs H1 H2. apply IH. now apply (suffix_size_decrease H2 H1).
 Defined.
 
 
-(** * Prefix *)
+(** * Codeable Class **)
 
-Definition prefix (X : Type) (xs ys : list X) :=
-  exists n : nat, firstn n ys = xs.
+Definition encoding_function (X : Type) := X -> list bool.
 
-Lemma prefix_full (X : Type) (xs : list X) :
-  prefix xs xs.
-Proof. exists (|xs|). apply List.firstn_all. Qed.
+Definition decoding_output (X : Type) (string : list bool) :=
+  option (X * {rest : list bool & suffix rest string}).
 
-Lemma prefix_app (X : Type) (xs ys zs : list X) :
-  prefix xs ys -> prefix xs (ys ++ zs).
+Definition decoding_output_proj (X : Type) :=
+  option (X * list bool).
+
+Definition decoding_function (X : Type) :=
+  forall string : list bool, decoding_output X string.
+
+Definition decoding_output_project (X : Type) (string : list bool) : decoding_output X string -> decoding_output_proj X.
+Proof. destruct 1; [ | apply None]. destruct p. apply Some. constructor. apply x. apply (projT1 s). Defined.
+
+Class codeable (X : Type) :=
+  {
+    encode : encoding_function X;
+    decode : decoding_function X;
+    encode_injective : forall (v1 v2 : X) (r1 r2 : list bool), encode v1 ++ r1 = encode v2 ++ r2 -> v1 = v2 /\ r1 = r2;
+    encode_decode : forall (string : list bool) v rest, decode string = Some (v, rest) -> encode v ++ (projT1 rest) = string;
+    decode_encode : forall (v : X) (rest : list bool),
+        match (decode (encode v ++ rest)) with
+        | Some (v', rest') => v = v' /\ projT1 rest' = rest
+        | None => False
+        end;
+  }.
+
+
+(** * Basic Encoding Functions *)
+
+Fixpoint encode_list (X : Type) (encode_entries : encoding_function X) (xs : list X) : list bool.
 Proof.
-  intros (n&<-).
-  decide (n < length ys) as [E|E'].
-  - exists (n). rewrite List.firstn_app.
-    replace (n - (| ys |)) with 0 by omega. cbn. rewrite List.app_nil_r. reflexivity.
-  - assert (|ys| <= n) as E by omega.
-    rewrite List.firstn_all2; auto. exists (|ys|). rewrite List.firstn_app.
-    replace ((| ys |) - (| ys |)) with 0 by omega. cbn. rewrite List.app_nil_r. apply List.firstn_all.
-Qed.
+  destruct xs.
+  - apply (false :: nil).
+  - apply (cons true). apply app. apply (encode_entries x). apply (encode_list X encode_entries xs).
+Defined.
 
-Lemma prefix_transitive (X : Type) (xs ys zs : list X) :
-  prefix xs ys -> prefix ys zs -> prefix xs zs.
-Proof. intros (n1&H1) (n2&H2). subst. exists (Nat.min n1 n2). now rewrite List.firstn_firstn. Qed.
+Definition encode_sum (X Y : Type) (encode_left : encoding_function X) (encode_right : encoding_function Y) (v : X + Y) : list bool.
+Proof.
+  destruct v.
+  - apply (true  :: encode_left  x).
+  - apply (false :: encode_right y).
+Defined.
+
+Definition encode_pair (X Y : Type) (encode_left : encoding_function X) (encode_right : encoding_function Y) (v : X * Y) : list bool.
+Proof. destruct v as (a,b). apply (encode_left a ++ encode_right b). Defined.
+  
+Definition encode_unit := fun _ : unit => @nil bool.
 
 
-(** * Decoding *)
+(** * Basic Decoding Functions *)
 
 Ltac invalid_encoding := apply None.
 
+(** List decoding *)
 
-Definition decoding_output (e : codtype) (string : list codsig) :=
-  option (codtype_to_type e * {rest : list codsig & suffix rest string}).
-
-Definition decoding_output_proj (e : codtype) :=
-  option (codtype_to_type e * list codsig).
-
-Definition decoding_function (e : codtype) :=
-  forall string : list codsig, decoding_output e string.
-
-Definition decoding_output_project (e : codtype) (string : list codsig) : decoding_output e string -> decoding_output_proj e.
-Proof. destruct 1; [ | apply None]. destruct p. apply Some. constructor. apply c. apply (projT1 s). Defined.
-
-
-Lemma suffix_skip' (X : Type) (x : X) (xs : list X) :
-  suffix xs (x :: xs).
-Proof. apply suffix_skip, suffix_full. Qed.
-
-Lemma decode_list'_helper1 (e : codtype) (x : codsig) (string : list codsig) (ss : list codsig)
-      (Rest1 : {rest : list codsig & suffix rest ss}) :
+Lemma decode_list'_helper1 (x : bool) (string : list bool) (ss : list bool)
+      (Rest1 : {rest : list bool & suffix rest ss}) :
   string = x :: ss -> suffix (projT1 Rest1) string.
 Proof. intros ->. destruct Rest1; cbn. now apply suffix_skip. Qed.
 
-Lemma decode_list'_helper2 (e : codtype) (x : codsig) (string : list codsig) (ss : list codsig)
-      (Rest2 : {rest : list codsig & suffix rest ss}) :
+Lemma decode_list'_helper2 (x : bool) (string : list bool) (ss : list bool)
+      (Rest2 : {rest : list bool & suffix rest ss}) :
       string = x :: ss -> projT1 Rest2 <> string.
-Proof. intros ->. destruct Rest2; cbn. intros ->. now apply suffix_put in s. Qed.
+Proof. intros ->. destruct Rest2; cbn. intros ->. eapply suffix_put; eauto. Qed.
 
-Lemma decode_list'_helper3 (e : codtype) (x : codsig) (string : list codsig) (ss : list codsig)
-      (Rest1 : {rest : list codsig & suffix rest ss})
-      (Rest2 : {rest : list codsig & suffix rest (projT1 Rest1)}) :
-  {rest : list codsig & suffix rest (x :: ss)}.
+Lemma decode_list'_helper3 (x : bool) (string : list bool) (ss : list bool)
+      (Rest1 : {rest : list bool & suffix rest ss})
+      (Rest2 : {rest : list bool & suffix rest (projT1 Rest1)}) :
+  {rest : list bool & suffix rest (x :: ss)}.
 Proof.
   destruct Rest1 as (rest1, HRest1). destruct Rest2 as (rest2, HRest2). cbn in *.
   exists rest2. apply suffix_skip. eapply suffix_transitive; eauto.
 Defined.
 
-(* Dont ask how long this took *)
-Fixpoint decode_list' (e : codtype) (decodeEntries : decoding_function e) (string : list codsig)
+Fixpoint decode_list' (X : Type) (decodeEntries : decoding_function X) (string : list bool)
          (ind : suffix_induction string) { struct ind } :
-  option (list (codtype_to_type e) * {rest : list codsig & suffix rest string }) :=
+  option (list X * {rest : list bool & suffix rest string }) :=
   let E := eq_refl : string = string in
   (match string as string'
          return
          (string = string' ->
-          option (list (codtype_to_type e) * {rest : list codsig & suffix rest string' })) with
+          option (list X * {rest : list bool & suffix rest string' })) with
    | nil => fun E0 : string = [] => None
    | true  :: ss => fun E0 : string = true :: ss =>
                      match (decodeEntries ss) with
@@ -297,54 +195,263 @@ Fixpoint decode_list' (e : codtype) (decodeEntries : decoding_function e) (strin
                      | Some (dec1, Rest1) =>
                        match ind with
                        | suffix_induction_con H => 
-                         match (@decode_list' e decodeEntries (projT1 Rest1) (H (projT1 Rest1)
-                                                                                (decode_list'_helper1 e Rest1 E0)
-                                                                                (decode_list'_helper2 e E0)
+                         match (@decode_list' X decodeEntries (projT1 Rest1) (H (projT1 Rest1)
+                                                                                (decode_list'_helper1 Rest1 E0)
+                                                                                (decode_list'_helper2 E0)
                                )) with
                          | None => None
                          | Some (dec2, Rest2) =>
-                           Some (dec1 :: dec2, @decode_list'_helper3 e true string ss Rest1 Rest2)
+                           Some (dec1 :: dec2, @decode_list'_helper3 true string ss Rest1 Rest2)
                          end
                        end
                      end
    | false :: ss => fun E0 : string = false :: ss => Some (nil, existT _ ss (suffix_skip' _ _))
    end) E.
 
-Definition decode_list (e : codtype) (decodeEntries : decoding_function e)
-           (string : list codsig) :=
-  @decode_list' e decodeEntries string (suffix_induction_provider string).
+Definition decode_list (X : Type) (decodeEntries : decoding_function X)
+           (string : list bool) :=
+  @decode_list' X decodeEntries string (suffix_induction_provider string).
 
 
-Fixpoint decode (t : codtype) (string : list codsig) :
-  option (codtype_to_type t * {rest : list codsig & suffix rest string}).
+Definition decode_pair (X Y : Type) (decode1 : decoding_function X) (decode2 : decoding_function Y) (string : list bool) :
+  option ((X * Y) * {rest : list bool & suffix rest string}).
 Proof.
-  destruct t; cbn in *.
-  - (* tuple *)
-    pose proof (decode t1) as decode1. pose proof (decode t2) as decode2.
-    destruct (decode1 string) as [ (dec1, (rest1, HRest1)) | ]; [ | invalid_encoding].
-    destruct (decode2 rest1)  as [ (dec2, (rest2, Hrest2)) | ]; [ | invalid_encoding].
-    do 2 constructor. constructor. apply dec1. apply dec2. exists rest2. eapply suffix_transitive; eauto.
-  - (* list *)
-    apply (decode_list'). unfold decoding_function. hnf. now apply decode. apply suffix_induction_provider.
-  - (* sum *)
-    pose proof (decode t1) as decode1. pose proof (decode t2) as decode2.
-    destruct string as [ | s ss].
-    + invalid_encoding.
-    + destruct s eqn:E.
-      * (* Inl = true *)
-        destruct (decode1 ss) as [ (dec, (rest, HRest)) | ]; [ | invalid_encoding].
-        constructor. constructor. left.  apply dec. exists rest. now apply suffix_skip.
-      * (* Inr = false *)
-        destruct (decode2 ss) as [ (dec, (rest, HRest)) | ]; [ | invalid_encoding].
-        constructor. constructor. right. apply dec. exists rest. now apply suffix_skip.
-  - (* unit *)
-    do 2 constructor. constructor. exists string. apply suffix_full.
+  destruct (decode1 string) as [ (dec1, (rest1, HRest1)) | ]; [ | invalid_encoding].
+  destruct (decode2 rest1)  as [ (dec2, (rest2, Hrest2)) | ]; [ | invalid_encoding].
+  do 2 constructor. constructor. apply dec1. apply dec2. exists rest2. eapply suffix_transitive; eauto.
+Defined.
+
+Definition decode_sum (X Y : Type) (decode1 : decoding_function X) (decode2 : decoding_function Y) (string : list bool) :
+  option ((X + Y) * {rest : list bool & suffix rest string}).
+Proof.
+  destruct string as [ | s ss].
+  - invalid_encoding.
+  - destruct s eqn:E.
+    + (* Inl = true *)
+      destruct (decode1 ss) as [ (dec, (rest, HRest)) | ]; [ | invalid_encoding].
+      constructor. constructor. left.  apply dec. exists rest. now apply suffix_skip.
+    + (* Inr = false *)
+      destruct (decode2 ss) as [ (dec, (rest, HRest)) | ]; [ | invalid_encoding].
+      constructor. constructor. right. apply dec. exists rest. now apply suffix_skip.
+Defined.
+
+Definition decode_unit (string : list bool) : option (unit * {rest : list bool & suffix rest string}).
+  do 2 constructor. constructor. exists string. apply suffix_full.
 Defined.
 
 
-(** * Encode and decode *) 
+(** * Basic Coding Instances *) 
 
-(** Test *)
+(** Lists **)
+
+Lemma encode_injective_list (X : Type) (e1 : codeable X) :
+  forall (v1 v2 : list X) (r1 r2 : list bool), encode_list encode v1 ++ r1 = encode_list encode v2 ++ r2 -> v1 = v2 /\ r1 = r2.
+Proof.
+  intros xs. induction xs as [ | x xs IH]; intros y2 r1 r2 H; cbn in *.
+  + destruct y2; cbn in *; try congruence. now inv H.
+  + destruct y2 as [ | y ys]; cbn in *; auto.
+    * congruence.
+    * inv H. rewrite <- !app_assoc in H1. apply encode_injective in H1. destruct H1 as (->&H1). apply IH in H1. intuition; congruence.
+Qed.
+
+Lemma encode_decode_list (X : Type) (e : codeable X) (string : list bool) ls rest :
+  decode_list decode string = Some (ls, rest) -> encode_list encode ls ++ (projT1 rest) = string.
+Proof.
+  unfold decode_list.
+  generalize (suffix_induction_provider string) as ind.
+  intros ind. revert ls rest. induction ind as [xs H IH]; intros ls rest H1.
+  cbn in *.
+  destruct xs as [ | x ss] eqn:E; try discriminate.
+  destruct x; cbn in *.
+  - destruct (decode ss) as [(dec1, Rest1)| ] eqn:E2; try discriminate; cbn in *.
+    destruct (decode_list' decode
+                           (H (projT1 Rest1)
+                              (decode_list'_helper1 Rest1 eq_refl)
+                              (decode_list'_helper2 eq_refl)))
+      as [(dec2, Rest2)| ] eqn:E3; try discriminate. inv H1.
+    specialize (IH _ _ _ _ _ E3).
+    destruct Rest1, Rest2. cbn in *. f_equal.
+    rewrite <- app_assoc. rewrite IH.
+    erewrite <- encode_decode; eauto.
+    cbn. reflexivity.
+  - inv H1. cbn. reflexivity.
+Qed.
+
+
+Lemma decode_encode_list (X : Type) (e : codeable X) :
+  forall (v : list X) (rest : list bool),
+    match (decode_list decode (encode_list encode v ++ rest)) with
+    | Some (v', rest') => v = v' /\ projT1 rest' = rest
+    | None => False
+    end.
+Proof.
+  intros v. induction v as [ | v vs IH]; intros rest.
+  - cbn. auto.
+  - cbn in *. rewrite <- !app_assoc in *.
+    pose proof (decode_encode v (encode_list encode vs ++ rest)) as E1'.
+    destruct (decode (encode v ++ encode_list encode vs ++ rest)) as [(dec1&rest1&HRest1)| ] eqn:E1; cbn; auto.
+    cbn in E1'. destruct E1' as (->&->).
+    specialize (IH rest).
+    destruct (encode_list encode vs ++ rest); auto.
+    destruct b; cbn in *; auto.
+    + destruct (decode l); auto. destruct p, s; cbn in *; auto.
+      destruct x0; cbn in *; auto. destruct b; cbn in *; auto. admit. admit.
+    + now destruct IH as (->&->).
+Admitted.
+
+Instance I_list (X : Type) (e1 : codeable X) : codeable (list X).
+Proof.
+  split with (encode := encode_list encode) (decode := decode_list decode).
+  - apply encode_injective_list.
+  - apply encode_decode_list.
+  - apply decode_encode_list.
+Defined.
+
+
+(** Pair *)
+
+Lemma encode_injective_pair (X Y : Type) (e1 : codeable X) (e2 : codeable Y) :
+  forall (v1 v2 : X * Y) (r1 r2 : list bool), encode_pair encode encode v1 ++ r1 = encode_pair encode encode v2 ++ r2 -> v1 = v2 /\ r1 = r2.
+Proof.
+  intros (a1, b1) (a2, b2) r1 r2 H. unfold encode_pair in *. rewrite <- !app_assoc in H.
+  apply encode_injective in H as (->&H). apply encode_injective in H as (->&->). auto.
+Qed.
+
+Lemma encode_decode_pair (X Y : Type) (e1 : codeable X) (e2 : codeable Y) (string : list bool) (v : X * Y) rest :
+  decode_pair decode decode string = Some (v, rest) -> encode_pair encode encode v ++ (projT1 rest) = string.
+Proof.
+  intros H. destruct v as (a, b).
+  unfold encode_pair, decode_pair in *.
+  destruct (decode string) as [(cod1, (rest1, HRest1))| ] eqn:E1; cbn in *; try discriminate.
+  destruct (decode rest1) as [(cod2, (rest2, HRest2))| ] eqn:E2; cbn in *; try discriminate.
+  inv H. cbn in *.
+  pose proof (@encode_decode X e1) as IH1. pose proof (@encode_decode Y e2) as IH2.
+  specialize (IH1 _ _ _ E1). cbn in *. specialize (IH2 _ _ _ E2). cbn in *.
+  subst. symmetry. now apply app_assoc.
+Qed.
+
+Lemma decode_encode_pair (X Y : Type) (e1 : codeable X) (e2 : codeable Y) :
+  forall (v : X * Y) (rest : list bool),
+    match (decode_pair decode decode (encode_pair encode encode v ++ rest)) with
+    | Some (v', rest') => v = v' /\ projT1 rest' = rest
+    | None => False
+    end.
+Proof.
+  intros (a, b) rest. unfold decode_pair, encode_pair.
+  rewrite <- app_assoc in *.
+  pose proof (decode_encode a (encode b ++ rest)) as E'.
+  destruct (decode (encode a ++ encode b ++ rest)) as [(dec1&rest1&Hrest1)| ] eqn:E; cbn in *.
+  - destruct E' as (->&->).
+    pose proof (decode_encode b rest) as E2'.
+    destruct (decode (encode b ++ rest) ) as [(dec2&rest2&Hrest2)| ] eqn:E2; cbn in *.
+    + destruct E2' as (->&->). auto.
+    + auto.
+  - auto.
+Qed.
+
+Instance I_pair (X Y : Type) (e1 : codeable X) (e2 : codeable Y) : codeable (X * Y).
+Proof.
+  split with (encode := encode_pair encode encode) (decode := decode_pair decode decode).
+  - apply encode_injective_pair.
+  - apply encode_decode_pair.
+  - apply decode_encode_pair.
+Defined.
+
+
+(** Sum **)
+
+Lemma encode_injective_sum (X Y : Type) (e1 : codeable X) (e2 : codeable Y) :
+  forall (v1 v2 : X + Y) (r1 r2 : list bool), encode_sum encode encode v1 ++ r1 = encode_sum encode encode v2 ++ r2 -> v1 = v2 /\ r1 = r2.
+Proof.
+  intros [v1|v1] [v2|v2] r1 r2; unfold encode_sum; intros H1; cbn in *; inv H1; apply encode_injective in H0; intuition; congruence.
+Qed.
+
+Lemma encode_decode_sum (X Y : Type) (e1 : codeable X) (e2 : codeable Y) (string : list bool) (v : X + Y) rest :
+  decode_sum decode decode string = Some (v, rest) -> encode_sum encode encode v ++ (projT1 rest) = string.
+Proof.
+  intros H. destruct v as [v1|v2].
+  + destruct string; try discriminate; cbn in *.
+    destruct b; try discriminate.
+    * destruct (decode string) eqn:E; cbn in *; try discriminate.
+      destruct p, s. inv H.
+      apply encode_decode in E. cbn in *. congruence.
+    * destruct (decode string) eqn:E; cbn in *; try discriminate.
+      destruct p, s. inv H.
+  + destruct string; try discriminate; cbn in *.
+    destruct b; try discriminate.
+    * destruct (decode string) eqn:E; cbn in *; try discriminate.
+      destruct p, s. inv H.
+    * destruct (decode string) eqn:E; cbn in *; try discriminate.
+      destruct p, s. inv H. apply encode_decode in E. cbn in *. congruence.
+Qed.
+
+Lemma decode_encode_sum (X Y : Type) (e1 : codeable X) (e2 : codeable Y) :
+  forall (v : X + Y) (rest : list bool),
+    match (decode_sum decode decode (encode_sum encode encode v ++ rest)) with
+    | Some (v', rest') => v = v' /\ projT1 rest' = rest
+    | None => False
+    end.
+Proof.
+  intros [a|a] rest.
+  - unfold decode_sum, encode_sum. cbn in *.
+    pose proof (decode_encode a rest) as E'.
+    destruct (decode (encode a ++ rest)) as [(dec1&rest1&Hreset1) | ]; auto.
+    intuition; congruence.
+  - unfold decode_sum, encode_sum. cbn in *.
+    pose proof (decode_encode a rest) as E'.
+    destruct (decode (encode a ++ rest)) as [(dec1&rest1&Hreset1) | ]; auto.
+    intuition; congruence.
+Qed.
+
+Instance I_sum (X Y : Type) (e1 : codeable X) (e2 : codeable Y) : codeable (X + Y).
+Proof.
+  split with (encode := encode_sum encode encode) (decode := decode_sum decode decode).
+  - apply encode_injective_sum.
+  - apply encode_decode_sum.
+  - apply decode_encode_sum.
+Defined.
+
+
+(** Unit **)
+
+Lemma encode_injective_unit :
+  forall (v1 v2 : unit) (r1 r2 : list bool), encode_unit v1 ++ r1 = encode_unit v2 ++ r2 -> v1 = v2 /\ r1 = r2.
+Proof. intros () () r1 r2. auto. Qed.
+
+Lemma encode_decode_unit (string : list bool) (v : unit) rest :
+  decode_unit string = Some (v, rest) -> encode_unit v ++ (projT1 rest) = string.
+Proof.
+  destruct v, rest. unfold decode_unit, encode_unit in *. intros H. inv H; cbn. reflexivity.
+Qed.
+
+Lemma decode_encode_unit :
+  forall (v : unit) (rest : list bool),
+    match (decode_unit (encode_unit v ++ rest)) with
+    | Some (v', rest') => v = v' /\ projT1 rest' = rest
+    | None => False
+    end.
+Proof.
+  destruct v, rest; unfold decode_unit, encode_unit in *; auto.
+Qed.
+
+Instance I_unit : codeable unit.
+Proof.
+  split with (encode := encode_unit) (decode := decode_unit).
+  - apply encode_injective_unit.
+  - apply encode_decode_unit.
+  - apply decode_encode_unit.
+Defined.
+
+
+
+(** Test Playground *)
+
+Compute decoding_output_project (decode (X := unit) (encode tt)).
+Compute decoding_output_project (decode (X := unit) (encode (tt, tt))).
+
+Compute (encode (X := list unit * (unit + unit) * (unit + unit)) ([tt;tt;tt], inr tt, inl tt)).
+Compute decoding_output_project (decode (X := list unit * (unit + unit) * (unit + unit)) (encode ([tt;tt;tt], inr tt, inl tt))).
+
 
 (*
 Compute decoding_output_project (decode (codunit) []).
@@ -365,59 +472,3 @@ Compute decoding_output_project
                          (@from_option codbool None, from_nat 3) ++ [true; true; false])).
 *)
 
-
-Lemma encode_decode_list (t : codtype) (string : list codsig) ls rest
-      (decode_entries : decoding_function t)
-      (encode_entries : encoding_function t) :
-  (forall string' v' rest',
-      decode_entries string' = Some (v', rest') -> encode_entries v' ++ (projT1 rest') = string'
-  ) ->
-  decode_list decode_entries string = Some (ls, rest) -> encode_list encode_entries ls ++ (projT1 rest) = string.
-Proof.
-  intros encode_decode_entries. unfold decode_list.
-  generalize (suffix_induction_provider string) as ind.
-  intros ind. revert ls rest. induction ind as [xs H IH]; intros ls rest H1.
-  cbn in *.
-  destruct xs as [ | x ss] eqn:E; try discriminate.
-  destruct x; cbn in *.
-  - destruct (decode_entries ss) as [(dec1, Rest1)| ] eqn:E2; try discriminate; cbn in *.
-    destruct (decode_list' decode_entries
-                           (H (projT1 Rest1)
-                              (decode_list'_helper1 t Rest1 eq_refl)
-                              (decode_list'_helper2 t eq_refl)))
-      as [(dec2, Rest2)| ] eqn:E3; try discriminate. inv H1.
-    specialize (IH _ _ _ _ _ E3).
-    destruct Rest1, Rest2. cbn in *. f_equal.
-    rewrite <- app_assoc. rewrite IH.
-    erewrite <- encode_decode_entries; eauto.
-    cbn. reflexivity.
-  - inv H1. cbn. reflexivity.
-Qed.
-
-Lemma encode_decode (t : codtype) (string : list codsig) v rest :
-  decode t string = Some (v, rest) -> encode v ++ (projT1 rest) = string.
-Proof.
-  revert string v rest. induction t; intros string v rest H.
-  - cbn in *. destruct v as (v1, v2).
-    destruct (decode t1 string) as [(cod1, (rest1, HRest1))| ] eqn:E1; cbn in *; try discriminate.
-    destruct (decode t2 rest1) as [(cod2, (rest2, HRest2))| ] eqn:E2; cbn in *; try discriminate.
-    inv H.
-    specialize (IHt1 _ _ _ E1). cbn in *.
-    specialize (IHt2 _ _ _ E2). cbn in *.
-    subst. now rewrite app_assoc.
-  - eapply encode_decode_list; eauto.
-  - cbn in *. destruct v as [v1|v2].
-    + destruct string; try discriminate; cbn in *.
-      destruct b; try discriminate.
-      * destruct (decode t1 string) eqn:E; cbn in *; try discriminate.
-        destruct p, s. inv H. specialize (IHt1 _ _ _ E). cbn in *. subst. reflexivity.
-      * destruct (decode t2 string) eqn:E; cbn in *; try discriminate.
-        destruct p, s. inv H.
-    + destruct string; try discriminate; cbn in *.
-      destruct b; try discriminate.
-      * destruct (decode t1 string) eqn:E; cbn in *; try discriminate.
-        destruct p, s. inv H.
-      * destruct (decode t2 string) eqn:E; cbn in *; try discriminate.
-        destruct p, s. inv H. specialize (IHt2 _ _ _ E). cbn in *. subst. reflexivity.
-  - cbn in *. destruct rest. cbn in *. now inv H.
-Qed.
